getting there, some inspiration from dot10.

dev2015/fsub2_wip.v
@@ -317,11 +317,14 @@ Inductive stp2: bool -> bool -> venv -> ty -> venv -> ty -> list (id*(venv*ty)) 
     stp2 false false G2 T3 G1 T1 GH n1 ->
     stp2 false false G1 T2 G2 T4 GH n2 ->
     stp2 m true G1 (TFun T1 T2) G2 (TFun T3 T4) GH (S (n1+n2))
-| stp2_mem: forall m G1 G2 T1 T2 T3 T4 GH n1 n2,
+| stp2_mem: forall G1 G2 T1 T2 T3 T4 GH n1 n2,
+    stp2 false false G2 T3 G1 T1 GH n1 ->
+    stp2 true true G1 T2 G2 T4 GH n2 ->
+    stp2 true true G1 (TMem T1 T2) G2 (TMem T3 T4) GH (S (n1+n2))
+| stp2_mem2: forall G1 G2 T1 T2 T3 T4 GH n1 n2,
     stp2 false false G2 T3 G1 T1 GH n1 ->
     stp2 false false G1 T2 G2 T4 GH n2 ->
-    stp2 m true G1 (TMem T1 T2) G2 (TMem T3 T4) GH (S (n1+n2))
-
+    stp2 false true G1 (TMem T1 T2) G2 (TMem T3 T4) GH (S (n1+n2))
 
 (* strong version, with precise/invertible bounds *)
 | stp2_strong_sel1: forall G1 G2 GX TX x T2 GH n1,
@@ -1970,9 +1973,13 @@ Proof.
     + SCase "top".
       apply stp2_reg1 in H. inversion H. eexists. eapply stp2_top. eassumption.
     + SCase "mem". subst.
-      assert (stpd2 false G3 T7 G1 T0 []) as A by solve [eapply stpd2_trans; eauto].
+      assert (stpd2 false G3 T7 G1 T0 []) as A. {
+        eapply stpd2_trans; eauto.
+      }
       inversion A as [na A'].
-      assert (stpd2 false G1 T4 G3 T8 []) as B by solve [eapply stpd2_trans; eauto].
+      assert (sstpd2 true G1 T4 G3 T8 []) as B. {
+        eapply IHn. eassumption. omega. eexists. eassumption.
+      }
       inversion B as [nb B'].
       eexists. eapply stp2_mem. apply A'. apply B'.
     + SCase "sel2". eexists. eapply stp2_strong_sel2. eauto. eauto. eapply stp2_transf. eauto. eauto.
@@ -2074,12 +2081,14 @@ Lemma invert_typ: forall venv vx T1 T2,
   exists GX TX,
     vx = (vty GX TX) /\
     stpd2 false venv T1 GX TX [] /\
-    stpd2 false GX TX venv T2 [].
+    sstpd2 true GX TX venv T2 [].
 Proof.
   intros. inversion H; ev; try solve by inversion. inversion H1.
   subst.
-  assert (stpd2 false venv0 T1 venv1 T0 []) as E1. eauto.
-  assert (stpd2 false venv1 T0 venv0 T2 []) as E2. eauto.
+  assert (stpd2 false venv0 T1 venv1 T0 []) as E1 by eauto.
+  assert (sstpd2 true venv1 T0 venv0 T2 []) as E2. {
+    eexists. eassumption.
+  }
   repeat eu. repeat eexists; eauto. 
 Qed.
 
@@ -2097,25 +2106,23 @@ Proof.
   - Case "top". eexists. eauto.
   - Case "bool". eexists. eauto.
   - Case "fun". eexists. eapply stp2_fun. eauto. eauto.
-  - Case "mem". eexists. eapply stp2_mem. eauto. eauto.
-  - Case "sel1".
-    (* TODO: val_type should take size bound parameter (if we do it like this) *)
-    (* alternative: sstp2_mem returns sstp2 *)
+  - Case "mem2".
+    eapply IHn in H2. eapply sstpd2_untrans in H2. inversion H2.
+    eexists. eapply stp2_mem. eauto. eauto. omega.
+  - Case "sel1". subst.
     eapply IHn in H4. eapply sstpd2_untrans in H4. eapply valtp_widen with (2:=H4) in H2.
-    eapply invert_typ in H2. ev. eu. eu. subst.
-    assert (x3 < n). admit. (* this is safe, because the val_tp was part of our argument *)
-    assert (x2 < n). admit.
+    eapply invert_typ in H2. ev. repeat eu. subst.
     assert (closed 0 (length ([]:aenv)) x1). eapply stp2_closed2; eauto.
-    assert (sstpd2 true x0 x1 G2 T2 []). eapply sstpd2_untrans. eapply IHn. eauto. omega.
-    eu. eexists. eapply stp2_strong_sel1. eauto. eauto. eauto. omega.
+    eexists. eapply stp2_strong_sel1. eauto. eauto. eauto. omega.
   - Case "sel2".
     eapply IHn in H4. eapply sstpd2_untrans in H4. eapply valtp_widen with (2:=H4) in H2.
-    eapply invert_typ in H2. ev. eu. eu. subst.
-    assert (x3 < n). admit. (* this is safe, because the val_tp was part of our argument *)
-    assert (x2 < n). admit.
+    eapply invert_typ in H2. ev. repeat eu. subst.
     assert (closed 0 (length ([]:aenv)) x1). eapply stp2_closed2; eauto.
-    assert (sstpd2 false G1 T1 x0 x1 []). eapply IHn. eauto. omega.
-    eu. eexists. eapply stp2_strong_sel2. eauto. eauto. eauto. omega.
+    assert (sstpd2 false G1 T1 x0 x1 []) as A. {
+      eapply IHn. eassumption. (* x2 < n *) admit.
+    }
+    inversion A as [na A'].
+    eexists. eapply stp2_strong_sel2. eauto. eauto. eauto. omega.
   - Case "selx".
     eexists. eapply stp2_strong_selx. eauto. eauto. 
   - Case "selh1". inversion H1. 
